Support expression matching outside MetaM

lib/ClausalExtraction/ArithTheory/ArithM.lean
@@ -54,21 +54,23 @@ instance : Add IntExpr where
 
 end IntExpr
 
--- Create a nat lit as an int
-def natLitAsIntExpr (n:Nat) : IntExpr :=
-  let z := mkRawNatLit n
+-- Create a nat as an int
+def mkOfNat (n:Expr) : IntExpr :=
   let ofNat := mkConst ``OfNat.ofNat [levelZero]
   let inst := mkConst ``Int.instOfNatInt
-  IntExpr.mk (mkAppN ofNat #[intExpr, z, mkApp inst z])
+  IntExpr.mk (mkAppN ofNat #[intExpr, n, mkApp inst n])
+
+-- Create a nat lit as an int
+def natLitAsIntExpr (n:Nat) : IntExpr := mkOfNat (mkRawNatLit n)
 
 def mkIntLit : Int → IntExpr
 | Int.ofNat n => natLitAsIntExpr n
 | Int.negSucc n => IntExpr.mk (mkApp intNegConst (natLitAsIntExpr (n+1)))
 
 instance : Coe Int IntExpr where
-  coe := fun x => mkIntLit x
+  coe := mkIntLit
 
-def intZeroExpr : IntExpr := natLitAsIntExpr 0
+def intZeroExpr : IntExpr := mkIntLit 0
 
 private def intNonNegExpr : Expr := mkConst ``Int.NonNeg
 def mkIntNonNegExpr (e:Expr) : Expr := mkApp intNonNegExpr e
@@ -81,58 +83,180 @@ end ExpressionUtils
 -- Represents a polynomial.
 structure Poly where
   -- Poly should be a sorted array of non-zero integers and variable pairs.
-  -- The
   elements : Array (Int × TheoryVar)
   deriving BEq, Hashable, Repr
 
 namespace Poly
 
 -- | Create polynomial denoting constant zero.
-def zero : Poly := ⟨#[]⟩
-
-instance : Inhabited Poly := ⟨zero⟩
+protected def const (z:Int) : Poly := ⟨#[(z, ⟨0⟩)]⟩
 
 -- | Create polynomial denoting constant zero.
-protected def one : Poly := ⟨#[(1, ⟨0⟩)]⟩
+protected def zero : Poly := Poly.const 0
+
+-- | Create polynomial denoting constant zero.
+protected def one : Poly := Poly.const 1
+
+instance : Inhabited Poly := ⟨Poly.zero⟩
+
+-- | Create polynomial denoting constant zero.
+-- protected def one : Poly := ⟨#[(1, ⟨0⟩)]⟩
+
+def addc : Poly → Int → Poly
+| ⟨a⟩, q =>
+  let (p,v) := a.get! 0
+  ⟨a.set! 0 (p+q, v)⟩
 
 -- | @add p i _ v@ returns poly denoting @p + i*v@.
-def add : ∀(p:Poly) (m:Int), TheoryVar → Poly
+def add : Poly → Int → TheoryVar → Poly
 | ⟨a⟩, q, v =>
   let rec loop : ∀(i : Nat), Poly
-      | 0 => ⟨a.insertAt 0 (q, v)⟩
+      | 0 => ⟨a.insertAt 1 (q, v)⟩
       | Nat.succ i =>
-        let (p,u) := a[i]
-        if u < v then
-          ⟨a.insertAt (i+1) (q,v)⟩
-        else if v < u then
+        let (p,u) := a[i+1]
+        if v < u then
           loop i
+        else if u < v then
+          ⟨a.insertAt (i+2) (q,v)⟩
         else -- v = u
           let q := p+q
           if q = 0 then
-            ⟨a.eraseIdx i⟩
+            ⟨a.eraseIdx (i+1)⟩
           else
-            ⟨a.set! i (q,v)⟩
-  loop a.size
+            ⟨a.set! (i+1) (q,v)⟩
+  loop (a.size-1)
 
 protected def toString : Poly → String
 | ⟨a⟩ =>
   let scalarProd : Int × TheoryVar → String
         | (m,v) => s!"{m}*{v}"
   let firstScalarProd : Int × TheoryVar → String
-        | (m, ⟨0⟩) => toString m
-        | p => scalarProd p
+        | (m, _) => toString m
   let polyIns := λ(e:String) h => s!"{e} + {scalarProd h}"
   a[1:].foldl polyIns (firstScalarProd a[0])
 
 instance : ToString Poly where
   toString := Poly.toString
 
+def scalarProd (f: v → IO IntExpr) : Int × v → IO IntExpr
+| (m,  v) => do IntExpr.mk (mkAppN intMulConst #[m, ← f v])
+
+-- | Create an reflexivity proof from the int expression.
+def mkIntRefl (e:IntExpr) : Expr := mkApp (mkApp (mkConst ``rfl [levelOne]) intExpr) e
+
+-- | Map polynomial to expression given mapping from variables
+-- to expressions.
+-- The optional parameter allowss this to to only take the first n elements.
+protected
+def expr (poly:Poly) (f: TheoryVar → IO IntExpr) (limit: optParam Nat (poly.elements.size - 1)) : IO IntExpr := do
+  if poly.elements.size = 0 then
+    panic! "Empty polyExpr"
+  if limit ≥ poly.elements.size then
+    panic! "polyExpr given bad limit."
+  let mut e : IntExpr ← poly.elements[0].fst
+  for p in poly.elements[1:limit+1] do
+    e := e + (← scalarProd f p)
+  pure e
+
+private
+theorem polyProofAddContextLemma {c x a:Int} (h:x + c = a) (y:Int)
+  : (x + y) + c = a + y := by
+  simp [h.symm, Int.add_assoc, Int.add_comm y c]
+
+-- polyProofAddContext s x c a h poly idx where h is a proof of "x + c = a" returns
+-- a proof "(x + poly[idx] + poly[idx+1] + ..) + c = a + poly[idx] + poly[idx+1] + .."
+private
+def polyProofAddContext (f:TheoryVar → IO IntExpr) (x c a:IntExpr) (h:Expr) (poly:Poly) (idx:Nat) : IO Expr := do
+  let mut x := x
+  let mut a := a
+  let mut h := h
+  let pr := mkApp (mkConst ``polyProofAddContextLemma) c
+  for p in poly.elements[idx:] do
+    let y ← scalarProd f p
+    h := mkAppN pr #[x, a, h, y]
+    x := x + y
+    a := a + y
+  pure h
+
+section Lemmas
+
+private
+theorem sum0Lemma (p q v:Int) : p*v + q*v = (p+q)*v := Eq.symm (Int.add_mul _ _ _)
+
+private
+theorem sumLemma (r p q v:Int) : (r + p*v) + q*v = r + (p+q)*v := by
+  apply Eq.trans (Int.add_assoc r _ _)
+  apply congrArg (fun y => r + y)
+  exact sum0Lemma _ _ _
+
+private
+theorem cancel0Lemma {p q:Int} (h : p+q = 0) (v:Int) : p*v + q*v = 0 := by
+  apply Eq.trans (sum0Lemma p q v)
+  exact @Eq.substr Int (λx => x * v = 0) _ _ h (Int.zero_mul v)
+
+example        : (64:Int) + -64 = 0   := @cancel0Lemma (64) (-64) (@rfl Int 0) 1
+example        : (-64:Int) + 64 = 0   := @cancel0Lemma (-64) (64) (@rfl Int 0) 1
+example (v:Int): -64 * v + 64 * v = 0 := @cancel0Lemma (-64) 64   (@rfl Int 0) v
+example (v:Int): 64 * v + -64 * v = 0 := @cancel0Lemma (64) (-64) (@rfl Int 0) v
+
+private
+theorem cancelLemma (r p q v:Int) (h : p+q = 0) : (r + p*v) + q*v = r := by
+  apply Eq.trans (Int.add_assoc r _ _)
+  exact Eq.trans (cancel0Lemma h v ▸ rfl) (Int.add_zero r)
+
+end Lemmas
+
+def addcProof (f:TheoryVar → IO IntExpr) (poly:Poly) (c:Int) (g:c ≠ 0) : IO Expr := do
+  let x := poly.elements[0].fst
+  let a := x + c
+  let h := mkIntRefl a
+  polyProofAddContext f x c a h poly 1
+
+-- | @addProof f p m v@ returns proof showing that
+-- @p.expr + scalarProd f (m, v) = (p.add m v).expr@.
+def addProof (f:TheoryVar → IO IntExpr) : ∀(poly:Poly) (q:Int), q ≠ 0 → TheoryVar → IO Expr
+| poly, q, g, v => do
+  let c ← scalarProd f (q, v)
+  let rec loop : ∀(i : Nat), IO Expr
+      | 0 => do
+        -- Handle case where var is zero.
+        let x : IntExpr := poly.elements[0].fst
+        let a := x + c
+        let h := mkIntRefl a
+        polyProofAddContext f x c a h poly 1
+      | Nat.succ i => do
+        let (p,u) := poly.elements[i+1]
+        if v < u then
+          loop i
+        else if u < v then
+          let x ← poly.expr f (limit := i+1)
+          let a := x + c
+          let h := mkIntRefl a
+          polyProofAddContext f x c a h poly (i+2)
+        else -- v = u
+          if p+q = 0 then
+            let a ← poly.expr f (limit := i)
+            let x := a + (← scalarProd f (p,u))
+            let rflExpr := mkIntRefl intZeroExpr
+            -- Create proof: (a + -q*v) + q*v = a.
+            let h := mkAppN (mkConst ``cancelLemma) #[a, (-q : Int), q, ← f v, rflExpr]
+            polyProofAddContext f x c a h poly (i+2)
+          else
+            let r ← poly.expr f (limit := i)
+            let x := r + (←scalarProd f (p, u))
+            let a := r + (←scalarProd f (p+q, u))
+            let h := mkAppN (mkConst ``sumLemma) #[r, p, q, ←f v]
+            polyProofAddContext f x c a h poly (i+2)
+  loop (poly.elements.size - 1)
+
 end Poly
 
 -- Definition associated with a variable.
 inductive Decl
-  -- Theory variable is equal to the expression.
-| uninterp : Var → Decl
+  -- A int variable from another theory.
+| uninterpInt : Var → Decl
+  -- A nat variable from another theory.
+| uninterpNat : Var → Decl
   -- Theory variable is equal to polynomial.
 | poly : Poly → Decl
 deriving BEq, Hashable
@@ -140,13 +264,14 @@ deriving BEq, Hashable
 namespace Decl
 
 protected def toString : Decl → String
-| uninterp v => s!"uninterp {v}"
+| uninterpInt v => s!"{v}"
+| uninterpNat v => s!"ofNat {v}"
 | poly p => s!"poly {p}"
 
 instance : ToString Decl where
   toString := Decl.toString
 
-instance : Inhabited Decl := ⟨uninterp arbitrary⟩
+instance : Inhabited Decl := ⟨uninterpInt arbitrary⟩
 
 end Decl
 
@@ -174,41 +299,26 @@ end Pred
 def oneVar : TheoryVar := ⟨0⟩
 
 structure State : Type where
+
   exprMap : HashMap Decl TheoryVar := Std.mkHashMap.insert (Decl.poly Poly.one) oneVar
   vars : Array Decl := #[Decl.poly Poly.one]
   preds : Array Pred := #[]
 
-mutual
+section
 
 variable (r:IO.Ref State)
-variable (f: Var → IO IntExpr)
-
-partial def scalarProd : Int × TheoryVar → IO IntExpr
-| (m, ⟨0⟩) => m
-| (m,  v) => do IntExpr.mk (mkAppN intMulConst #[m, ← thvarExpr v])
-
--- | Map polynomial to expression given mapping from variables
--- to expressions.
--- The optional parameter allowss this to to only take the first n elements.
-partial def polyExpr (poly:Poly) (limit: optParam Nat (poly.elements.size)) : IO IntExpr := do
-  if limit > poly.elements.size then
-    panic! "polyExpr given bad limit."
-  if limit = 0 then
-    (0 : Int)
-  else do
-    let mut e ← scalarProd poly.elements[0]
-    for p in poly.elements[1:limit] do
-      e := e + (← scalarProd p)
-    pure e
+variable (f: Var → IO Expr)
 
 -- | Return Lean expression associated with IntExpr
 partial def thvarExpr (v:TheoryVar) : IO IntExpr := do
   let s ← r.get
   if p : v.toNat < s.vars.size then
     match s.vars.get ⟨v.toNat, p⟩  with
-    | Decl.uninterp v => do
-      f v
-    | Decl.poly p => polyExpr p
+    | Decl.uninterpInt v => do
+      IntExpr.mk <$> f v
+    | Decl.uninterpNat v => do
+      mkOfNat <$> f v
+    | Decl.poly p => p.expr (thvarExpr)
   else
     panic! s!"Invalid theory variable index {v} (max = {s.vars.size})"
 
@@ -217,7 +327,7 @@ end
 abbrev ArithM := ReaderT (IO.Ref State) SolverM
 
 -- | Return a theory variable associated with the given uninterpreted Lean expression.
-private def getVar (d:Decl) : ArithM TheoryVar := do
+def getTheoryVar (d:Decl) : ArithM TheoryVar := do
   let r ← read
   let s ← r.get
   match s.exprMap.find? d with
@@ -232,32 +342,19 @@ private def getVar (d:Decl) : ArithM TheoryVar := do
   return newVar
 
 -- | Return a theory variable associated with the given uninterpreted Lean expression.
-def getUninterpVar (v:Var) : ArithM TheoryVar := getVar (Decl.uninterp v)
-
--- | Return a theory variable associated with the given uninterpreted Lean expression.
-def getPolyVar (p:Poly) : ArithM TheoryVar := getVar (Decl.poly p)
-
-
-/-
--- | Assert a predicate holds using the given expression to refer to the
--- proof.
-def assertPred (origin:Option FVarId) (userName:Name) (proof:Expr) (prop:Pred) : ArithM Solver Unit := do
-  let a := { origin := origin, name := userName, proof := proof, prop := prop }
-  modifyGet fun s => ((), { s with assertions := s.assertions.push a })
--/
+def getPolyVar (p:Poly) : ArithM TheoryVar := getTheoryVar (Decl.poly p)
 
 def getThvarExpr (v:TheoryVar) : ArithM IntExpr := do
   let svc ← (read : SolverM _)
-  let f (v:Var) : IO IntExpr := IntExpr.mk <$> svc.varExpr v
   let r ← read
-  thvarExpr r f v
+  thvarExpr r svc.varExpr v
 
 -- | Return expression associated with in solver.
 def getPolyExpr (poly:Poly) : ArithM IntExpr := do
   let svc ← (read : SolverM _)
-  let f (v:Var) : IO IntExpr := IntExpr.mk <$> svc.varExpr v
   let r ← read
-  polyExpr r f poly
+  let f (v:TheoryVar) : IO IntExpr := thvarExpr r svc.varExpr v
+  poly.expr f
 
 def getTheoryPred (p:Pred) : ArithM TheoryPred := do
   let r ← read
@@ -269,7 +366,7 @@ def getTheoryPred (p:Pred) : ArithM TheoryPred := do
   pure n
 
 def mthvarExpr (r: IO.Ref State) (f : Var → IO Expr)  (thv : TheoryVar) : IO Expr := do
-  IntExpr.toExpr <$> thvarExpr r (fun v => IntExpr.mk <$> f v) thv
+  IntExpr.toExpr <$> thvarExpr r f thv
 
 def predExpr (r : IO.Ref State) (f : Var → IO Expr) (idx : TheoryPred) : IO Expr := do
   let s ← r.get
